Fixed ex6b

doc/tutorial/code/solutions/ex6b-sort-poly.fst
@@ -1,56 +1,63 @@
 module QuickSortPoly
 
+
 val mem: 'a -> list 'a -> Tot bool
 let rec mem a l = match l with
   | [] -> false
   | hd::tl -> hd=a || mem a tl
+
 
 val append : list 'a -> list 'a -> Tot (list 'a)
 let rec append l1 l2 = match l1 with
   | [] -> l2
   | hd :: tl -> hd :: append tl l2
 
+
+val append_mem:  l1:list 'a
+              -> l2:list 'a
+              -> Lemma (requires True)
+                       (ensures (forall a. mem a (append l1 l2) = (mem a l1 || mem a l2)))
+                       [SMTPat (append l1 l2)]
+let rec append_mem l1 l2 = match l1 with
+  | [] -> ()
+  | hd::tl -> append_mem tl l2
+
+
 val length: list 'a -> Tot nat
 let rec length l = match l with
   | [] -> 0
   | _ :: tl -> 1 + length tl
 
+
+(* Specification of sortedness according to some comparison function f *)
+val sorted: ('a -> 'a -> Tot bool) -> list 'a -> Tot bool
+let rec sorted f l = match l with
+    | [] -> true
+    | [x] -> true
+    | x::y::xs -> f x y && sorted f (y::xs)
+
+
 val partition: ('a -> Tot bool) -> list 'a -> Tot (list 'a * list 'a)
-let rec partition f = function 
+let rec partition f = function
   | [] -> [], []
-  | hd::tl -> 
-    let l1, l2 = partition f tl in
-    if f hd 
-    then hd::l1, l2
-    else l1, hd::l2
+  | hd::tl ->
+     let l1, l2 = partition f tl in
+     if f hd
+     then hd::l1, l2
+     else l1, hd::l2
+
 
 val partition_lemma: f:('a -> Tot bool)
                    -> l:list 'a
                    -> Lemma (requires True)
                             (ensures ((length (fst (partition f l)) + length (snd (partition f l)) = length l
-                                 /\ (forall x. mem x (fst (partition f l)) ==> f x)
-                                 /\ (forall x. mem x (snd (partition f l)) ==> not (f x))
-                                 /\ (forall x. mem x l = (mem x (fst (partition f l)) || mem x (snd (partition f l)))))))
-let rec partition_lemma f l = match l with 
-  | [] -> ()
-  | hd::tl -> partition_lemma f tl
+                                  /\ (forall x. mem x (fst (partition f l)) ==> f x)
+                                  /\ (forall x. mem x (snd (partition f l)) ==> not (f x))
+                                  /\ (forall x. mem x l = (mem x (fst (partition f l)) || mem x (snd (partition f l)))))))
+let rec partition_lemma f l = match l with
+    | [] -> ()
+    | hd::tl -> partition_lemma f tl
 
-(* Specification of sortedness according to some comparison function f *)
-val sorted: ('a -> 'a -> Tot bool) -> list 'a -> Tot bool
-let rec sorted f = function
-  | []
-  | [_] -> true
-  | x::y::tl -> f x y && sorted f (y::tl)
-
-val sorted_concat_lemma: l1:list int{sorted l1}
-                      -> l2:list int{sorted l2}
-                      -> pivot:int
-                      -> Lemma (requires ((forall y. mem y l1 ==> not (pivot <= y))
-                                       /\ (forall y. mem y l2 ==> pivot <= y)))
-                               (ensures (sorted (append l1 (pivot::l2))))
-                         [SMTPat (sorted (append l1 (pivot::l2)))]
-
-(* Use the same lemma about List.partition as previously. *)
 
 (* Defining a new predicate symbol *)
 opaque type total_order (a:Type) (f: (a -> a -> Tot bool)) =
@@ -58,27 +65,28 @@ opaque type total_order (a:Type) (f: (a -> a -> Tot bool)) =
     /\ (forall a1 a2. (f a1 a2 /\ a1<>a2)  <==> not (f a2 a1))  (* anti-symmetry *)
     /\ (forall a1 a2 a3. f a1 a2 /\ f a2 a3 ==> f a1 a3)        (* transitivity  *)
 
-val sorted_concat_lemma:  a:Type
-               ->  f:(a -> a -> Tot bool)
-               ->  l1:list a{sorted f l1}
-               ->  l2:list a{sorted f l2}
-               ->  pivot:a
-               ->  Lemma (requires (total_order a f
-                                    /\ (forall y. mem y l1 ==> not(f pivot y))
-                                    /\ (forall y. mem y l2 ==> f pivot y)))
-                         (ensures (sorted f (append l1 (pivot::l2))))
-                         [SMTPat (sorted f (append l1 (pivot::l2)))]
-let rec sorted_concat_lemma f l1 l2 pivot = match l1 with 
-  | [] -> ()
-  | hd::tl -> sorted_concat_lemma f tl l2 pivot
+val sorted_concat_lemma: a:Type
+                      -> f:(a -> a -> Tot bool)
+                      -> l1:list a{sorted f l1}
+                      -> l2:list a{sorted f l2}
+                      -> pivot:a
+                      -> Lemma (requires (total_order a f
+                                       /\ (forall y. mem y l1 ==> not (f pivot y))
+                                       /\ (forall y. mem y l2 ==> f pivot y)))
+                               (ensures (sorted f (append l1 (pivot::l2))))
+                               [SMTPat (sorted f (append l1 (pivot::l2)))]
+let rec sorted_concat_lemma f l1 l2 pivot = match l1 with
+    | [] -> ()
+    | hd::tl -> sorted_concat_lemma f tl l2 pivot
+
 
 val sort: f:('a -> 'a -> Tot bool){total_order 'a f}
-      ->  l:list 'a
-      ->  Tot (m:list 'a{sorted f m /\ (forall x. mem x l = mem x m)})
+       -> l:list 'a
+       -> Tot (m:list 'a{sorted f m /\ (forall i. mem i l = mem i m)})
               (decreases (length l))
-let rec sort f = function
+let rec sort f l = match l with
   | [] -> []
-  | pivot::tl -> 
-    let hi, lo  = partition (f pivot) tl in 
+  | pivot::tl ->
+    let hi, lo = partition (f pivot) tl in
     partition_lemma (f pivot) tl;
-    sort f (append lo (pivot::sort f hi))
+    append (sort f lo) (pivot::sort f hi)
